libcrux-ml-kem/proofs/fstar/extraction/Libcrux_ml_kem.Vector.Portable.Ntt.fsti
@@ -198,6 +198,13 @@ val ntt_multiply
         fun result ->
           let result:Libcrux_ml_kem.Vector.Portable.Vector_type.t_PortableVector = result in
           Spec.Utils.is_i16b_array 3328 result.f_elements /\
+          Spec.Utils.ntt_multiply_butterfly_post lhs.f_elements
+            rhs.f_elements
+            result.f_elements
+            zeta0
+            zeta1
+            zeta2
+            zeta3 /\
           (let nzeta0:i16 = mk_i16 0 -! zeta0 in
             let nzeta1:i16 = mk_i16 0 -! zeta1 in
             let nzeta2:i16 = mk_i16 0 -! zeta2 in
